LeanChess.lean
@@ -1,3 +1,4 @@
 import domain.Game
 import domain.Deep
 import domain.Lazier
+import domain.Semantics
